proof/correctness1024/Fq.ec
@@ -7,7 +7,7 @@ from JazzEC require import Array32.
 require import Montgomery.
 require import W16extra MLKEMFCLib.
 
-from CryptoSpecs require import GFq Correctness768.
+from CryptoSpecs require import GFq Correctness1024.
 
 import Zq.
 
@@ -26,7 +26,7 @@ clone import SignedReductions with
     proof RRinv by (rewrite /R qE  => />)
     proof qinv_bnd by (rewrite /R  => />).
 
-from JazzEC require import Jkem768.
+from JazzEC require import Jkem1024.
 
 lemma smod_W16 a:
   smod a W16.modulus = W16.smod (a %% W16.modulus)
@@ -80,7 +80,7 @@ proof. by conseq fqmul_old_ll (fqmul_old_corr_h _a _b). qed.
 
 
 lemma fqmul_corr_h _a _b: 
-   hoare[Jkem768.M(Jkem768.Syscall).__fqmul : 
+   hoare[Jkem1024.M(Jkem1024.Syscall).__fqmul : 
      to_sint a = _a /\ to_sint b = _b ==> to_sint res = SREDC (_a * _b)].
 proof.
 proc; wp; skip  => &hr [#] /= H H0.
@@ -89,10 +89,10 @@ rewrite smod_W32 smod_W32 smod_W16 W16.of_sintK /(`<<`) /sigextu32 /truncateu16 
 by rewrite W32.to_sintE W32.of_uintK W32.of_uintK W32.of_sintK qE /= !modz_dvd /R /=; smt().
 qed.
 
-lemma fqmul_ll : islossless Jkem768.M(Jkem768.Syscall).__fqmul by proc; islossless.
+lemma fqmul_ll : islossless Jkem1024.M(Jkem1024.Syscall).__fqmul by proc; islossless.
 
 lemma fqmul_corr _a _b :
-  phoare [Jkem768.M(Jkem768.Syscall).__fqmul : 
+  phoare [Jkem1024.M(Jkem1024.Syscall).__fqmul : 
      W16.to_sint a = _a /\ W16.to_sint b = _b ==> 
          W16.to_sint res = SREDC (_a * _b)] = 1%r.
 proof. by conseq fqmul_ll (fqmul_corr_h _a _b). qed.
@@ -194,7 +194,7 @@ qed.
 
 
 lemma barrett_reduce_corr_h _a :
-  hoare [Jkem768.M(Jkem768.Syscall).__barrett_reduce : 
+  hoare [Jkem1024.M(Jkem1024.Syscall).__barrett_reduce : 
      W16.to_sint a = _a  ==> 
          W16.to_sint res = BREDC _a 26].
 proof.
@@ -216,10 +216,10 @@ have ->: to_uint a{hr} - 65536 = to_uint a{hr} + (-1) * 65536; 1: by ring.
 by rewrite modzMDr; smt(W16.to_uint_cmp pow2_16).
 qed.
 
-lemma barrett_reduce_ll :  islossless Jkem768.M(Jkem768.Syscall).__barrett_reduce by proc; islossless.
+lemma barrett_reduce_ll :  islossless Jkem1024.M(Jkem1024.Syscall).__barrett_reduce by proc; islossless.
 
 lemma barrett_reduce_corr _a :
-  phoare [Jkem768.M(Jkem768.Syscall).__barrett_reduce : 
+  phoare [Jkem1024.M(Jkem1024.Syscall).__barrett_reduce : 
      W16.to_sint a = _a  ==> 
          W16.to_sint res = BREDC _a 26] = 1%r.
 proof. by conseq barrett_reduce_ll (barrett_reduce_corr_h _a). qed.
