proof/correctness768/avx2/MLKEM_InnerPKE_avx2_stack.ec
@@ -9,7 +9,7 @@ from Jasmin require import JModel_x86.
 from JazzEC require import Array32 Array33 Array64 Array148 Array256 Array768 Array960 Array128 Array1088 Array1152 Array1184 Array2304 Array2400.
 from JazzEC require import Array8 WArray32 WArray33 Array300 WArray64 WArray1184 WArray2400.
 
-from CryptoSpecs require import MLKEM InnerPKE.
+from CryptoSpecs require import MLKEM768 InnerPKE768.
 
 module Mix = {
   
@@ -346,9 +346,9 @@ qed.
 require import MLKEMFCLib MLKEM_PolyPolyVec_stack_bridges.
 
 
-import InnerPKE.
+import InnerPKE768.
 equiv mlkem_correct_kg_avx2_stack  : 
-M.__indcpa_keypair  ~ InnerPKE.kg_derand :
+M.__indcpa_keypair  ~ InnerPKE768.kg_derand :
 arg{1}.`3 = arg{2} ==> 
     res{2}.`2 = Array1152.init ("_.[_]" res{1}.`2) /\
     res{2}.`1.`1 = (init (fun (i : int) => res{1}.`1.[i]))%Array1152 /\
@@ -473,7 +473,7 @@ qed.
 
 
 equiv mlkem_correct_enc_avx2_stack  : 
-M.__indcpa_enc  ~ InnerPKE.enc_derand :
+M.__indcpa_enc  ~ InnerPKE768.enc_derand :
 arg{1}.`2 = arg{2}.`2 /\ arg{1}.`4 = arg{2}.`3 /\
    Array1152.init(fun i => arg{1}.`3.[i]) = arg{2}.`1.`1 /\
    Array32.init(fun i => arg{1}.`3.[i+1152]) = arg{2}.`1.`2 ==>
@@ -546,7 +546,7 @@ qed.
 
 
 equiv mlkem_correct_dec_avx2_stack  : 
-M.__indcpa_dec  ~ InnerPKE.dec :
+M.__indcpa_dec  ~ InnerPKE768.dec :
 arg{1}.`3 = arg{2}.`1 /\ 
 Array960.init(fun i => arg{1}.`2.[i]) = arg{2}.`2.`1 /\
 Array128.init(fun i => arg{1}.`2.[i+960]) = arg{2}.`2.`2  ==>
